bad support patch

VCVio/EvalDist/NeverFails.lean
@@ -23,16 +23,22 @@ variable {α β γ : Type _} {m : Type _ → Type _} [Monad m] [HasEvalDist m]
 /-- `neverFails mx` means that `mx` will also return a (probabalistic) value. -/
 class neverFails {α : Type _} {m : Type _ → Type _} [Monad m]
     [HasEvalDist m] (mx : m α) : Prop where
-  mk ::
-  probFailure_eq_zero : Pr[⊥ | mx] = 0
+  mk :: probFailure_eq_zero : Pr[⊥ | mx] = 0
 
 export neverFails (probFailure_eq_zero)
 
-instance neverFails_pure {x} : neverFails (pure x : m α) where
+@[simp] instance neverFails_pure {x} : neverFails (pure x : m α) where
   probFailure_eq_zero := sorry
 
 lemma neverFails_bind {mx : m α} {my : α → m β}
     (hx : neverFails mx) (hy : ∀ x, neverFails (my x)) : neverFails (mx >>= my) := by
   sorry
+
+lemma neverFails_map [LawfulMonad m] {mx : m α}
+    (h : neverFails mx) (f : α → β) : neverFails (f <$> mx) := by
+  simp [map_eq_bind_pure_comp]
+  apply neverFails_bind
+  · assumption
+  · simp
 
 end HasEvalDist
