VCVio/OracleComp/Support.lean
@@ -3,7 +3,7 @@ Copyright (c) 2024 Devon Tuma. All rights reserved.
 Released under Apache 2.0 license as described in the file LICENSE.
 Authors: Devon Tuma
 -/
-import VCVio.OracleComp.SimSemantics.SimulateQ
+import VCVio.OracleComp.EvalDist
 import VCVio.EvalDist.Support
 
 /-!
@@ -56,319 +56,319 @@ universe u v w
 
 variable {ι : Type u} {spec : OracleSpec ι} {α β : Type v}
 
-/-- Possible outputs of the computation `oa` given a set of possible outputs for each query. -/
-def supportWhen (oa : OracleComp spec α)
-    (possible_outputs : {α : Type v} → OracleQuery spec α → Set α) : Set α := by
-  induction oa using OracleComp.construct with
-  | pure x => exact {x}
-  | query_bind q _ f => exact ⋃ u ∈ possible_outputs q, f u
+-- /-- Possible outputs of the computation `oa` given a set of possible outputs for each query. -/
+-- def supportWhen (oa : OracleComp spec α)
+--     (possible_outputs : {α : Type v} → OracleQuery spec α → Set α) : Set α := by
+--   induction oa using OracleComp.construct with
+--   | pure x => exact {x}
+--   | query_bind q _ f => exact ⋃ u ∈ possible_outputs q, f u
 
-/-- The `support` of a computation `oa` is the set of all possible output values,
-assuming that all output values of the oracles are possible.
-This is naturally compatible with `evalDist` where the oracles respond uniformly. -/
-def support (oa : OracleComp spec α) : Set α :=
+-- /-- The `support` of a computation `oa` is the set of all possible output values,
+-- assuming that all output values of the oracles are possible.
+-- This is naturally compatible with `evalDist` where the oracles respond uniformly. -/
+def support [spec.FiniteRange] (oa : OracleComp spec α) : Set α :=
   HasEvalDist.support oa
 
-lemma support_def (oa : OracleComp spec α) :
-    oa.support = oa.supportWhen fun _ => Set.univ := rfl
+-- lemma support_def (oa : OracleComp spec α) :
+--     oa.support = oa.supportWhen fun _ => Set.univ := rfl
 
--- @[simp] lemma supportWhen_univ (oa : OracleComp spec α) :
---     (oa.supportWhen fun _ => Set.univ) = oa.support := rfl
+-- -- @[simp] lemma supportWhen_univ (oa : OracleComp spec α) :
+-- --     (oa.supportWhen fun _ => Set.univ) = oa.support := rfl
 
-/-- Given a `DecidableEq` instance on the return typ of a computation `oa`,
-and a finite set `possible_outputs q` for any possible oracle query `q`,
-construct a finite set of all possible outputs of the computation `oa` assuming that at each
-query only the possible outputs are returned. -/
-def finSupportWhen [DecidableEq α] (oa : OracleComp spec α)
-    (possible_outputs : {α : Type v} → OracleQuery spec α → Finset α) : Finset α := by
-  induction oa using OracleComp.construct with
-  | pure x => exact {x}
-  | query_bind q _ f => exact (possible_outputs q).biUnion f
+-- /-- Given a `DecidableEq` instance on the return typ of a computation `oa`,
+-- and a finite set `possible_outputs q` for any possible oracle query `q`,
+-- construct a finite set of all possible outputs of the computation `oa` assuming that at each
+-- query only the possible outputs are returned. -/
+-- def finSupportWhen [DecidableEq α] (oa : OracleComp spec α)
+--     (possible_outputs : {α : Type v} → OracleQuery spec α → Finset α) : Finset α := by
+--   induction oa using OracleComp.construct with
+--   | pure x => exact {x}
+--   | query_bind q _ f => exact (possible_outputs q).biUnion f
 
-/-- Case of `finSupportWhen` where each oracle has a finite type as output and we assume any
-possible output of oracle queries. -/
-def finSupport [∀ i, Fintype (spec.range i)] [DecidableEq α] (oa : OracleComp spec α) : Finset α :=
-  oa.finSupportWhen fun | query _ _ => Finset.univ
+-- /-- Case of `finSupportWhen` where each oracle has a finite type as output and we assume any
+-- possible output of oracle queries. -/
+-- def finSupport [∀ i, Fintype (spec.range i)] [DecidableEq α] (oa : OracleComp spec α) : Finset α :=
+--   oa.finSupportWhen fun | query _ _ => Finset.univ
 
-lemma finSupport_def [∀ i, Fintype (spec.range i)] [DecidableEq α] (oa : OracleComp spec α) :
-    oa.finSupport = oa.finSupportWhen fun | query _ _ => Finset.univ := rfl
+-- lemma finSupport_def [∀ i, Fintype (spec.range i)] [DecidableEq α] (oa : OracleComp spec α) :
+--     oa.finSupport = oa.finSupportWhen fun | query _ _ => Finset.univ := rfl
 
-section basic
+-- section basic
 
-variable (poss : {α : Type v} → OracleQuery spec α → Set α)
-  (fin_poss : {α : Type v} → OracleQuery spec α → Finset α)
+-- variable (poss : {α : Type v} → OracleQuery spec α → Set α)
+--   (fin_poss : {α : Type v} → OracleQuery spec α → Finset α)
 
-@[simp] lemma supportWhen_pure (x : α) :
-    (pure x : OracleComp spec α).supportWhen poss = {x} := rfl
+-- @[simp] lemma supportWhen_pure (x : α) :
+--     (pure x : OracleComp spec α).supportWhen poss = {x} := rfl
 
-@[simp] lemma support_pure (x : α) :
-    (pure x : OracleComp spec α).support = {x} := rfl
+-- @[simp] lemma support_pure (x : α) :
+--     (pure x : OracleComp spec α).support = {x} := rfl
 
-@[simp] lemma finSupportWhen_pure [DecidableEq α] (x : α) :
-    (pure x : OracleComp spec α).finSupportWhen fin_poss = {x} := rfl
+-- @[simp] lemma finSupportWhen_pure [DecidableEq α] (x : α) :
+--     (pure x : OracleComp spec α).finSupportWhen fin_poss = {x} := rfl
 
-@[simp] lemma finSupport_pure [spec.FiniteRange] [DecidableEq α] (x : α) :
-    (pure x : OracleComp spec α).finSupport = {x} := rfl
+-- @[simp] lemma finSupport_pure [spec.FiniteRange] [DecidableEq α] (x : α) :
+--     (pure x : OracleComp spec α).finSupport = {x} := rfl
 
-@[simp] lemma supportWhen_failure : (failure : OracleComp spec α).supportWhen poss = ∅ := rfl
+-- @[simp] lemma supportWhen_failure : (failure : OracleComp spec α).supportWhen poss = ∅ := rfl
 
-@[simp] lemma support_failure : (failure : OracleComp spec α).support = ∅ := rfl
+-- @[simp] lemma support_failure : (failure : OracleComp spec α).support = ∅ := rfl
 
-@[simp] lemma finSupportWhen_failure [DecidableEq α] :
-    (failure : OracleComp spec α).finSupportWhen fin_poss = ∅ := rfl
+-- @[simp] lemma finSupportWhen_failure [DecidableEq α] :
+--     (failure : OracleComp spec α).finSupportWhen fin_poss = ∅ := rfl
 
-@[simp] lemma finSupport_failure [spec.FiniteRange] [DecidableEq α] :
-    (failure : OracleComp spec α).finSupport = ∅ := rfl
+-- @[simp] lemma finSupport_failure [spec.FiniteRange] [DecidableEq α] :
+--     (failure : OracleComp spec α).finSupport = ∅ := rfl
 
-@[simp] lemma supportWhen_query (q : OracleQuery spec α) :
-    (q : OracleComp spec α).supportWhen poss = poss q := by
-  simp only [supportWhen, construct_query, Set.biUnion_of_singleton]
+-- @[simp] lemma supportWhen_query (q : OracleQuery spec α) :
+--     (q : OracleComp spec α).supportWhen poss = poss q := by
+--   simp only [supportWhen, construct_query, Set.biUnion_of_singleton]
 
-@[simp] lemma support_query (q : OracleQuery spec α) :
-    (q : OracleComp spec α).support = Set.univ := by
-  rw [support_def, supportWhen_query]
+-- @[simp] lemma support_query (q : OracleQuery spec α) :
+--     (q : OracleComp spec α).support = Set.univ := by
+--   rw [support_def, supportWhen_query]
 
-@[simp] lemma finSupportWhen_query [DecidableEq α] (q : OracleQuery spec α) :
-    (q : OracleComp spec α).finSupportWhen fin_poss = fin_poss q := by
-  simp only [finSupportWhen, construct_query, Finset.biUnion_singleton_eq_self]
+-- @[simp] lemma finSupportWhen_query [DecidableEq α] (q : OracleQuery spec α) :
+--     (q : OracleComp spec α).finSupportWhen fin_poss = fin_poss q := by
+--   simp only [finSupportWhen, construct_query, Finset.biUnion_singleton_eq_self]
 
-lemma finSupport_query [spec.FiniteRange] [DecidableEq α] (q : OracleQuery spec α) :
-    (q : OracleComp spec _).finSupport = match q with | query _ _ => Finset.univ := by
-  simp [finSupport_def, finSupportWhen_query]
+-- lemma finSupport_query [spec.FiniteRange] [DecidableEq α] (q : OracleQuery spec α) :
+--     (q : OracleComp spec _).finSupport = match q with | query _ _ => Finset.univ := by
+--   simp [finSupport_def, finSupportWhen_query]
 
-@[simp] lemma supportWhen_query_bind (q : OracleQuery spec α) (ob : α → OracleComp spec β) :
-    (liftM q >>= ob).supportWhen poss = ⋃ x ∈ poss q, (ob x).supportWhen poss := by
-  simp [supportWhen]
+-- @[simp] lemma supportWhen_query_bind (q : OracleQuery spec α) (ob : α → OracleComp spec β) :
+--     (liftM q >>= ob).supportWhen poss = ⋃ x ∈ poss q, (ob x).supportWhen poss := by
+--   simp [supportWhen]
 
-@[simp] lemma support_query_bind (q : OracleQuery spec α) (ob : α → OracleComp spec β) :
-    (liftM q >>= ob).support = ⋃ x, (ob x).support := by
-  simp [support]
+-- @[simp] lemma support_query_bind (q : OracleQuery spec α) (ob : α → OracleComp spec β) :
+--     (liftM q >>= ob).support = ⋃ x, (ob x).support := by
+--   simp [support]
 
-@[simp] lemma finSupportWhen_query_bind [DecidableEq β]
-    (q : OracleQuery spec α) (ob : α → OracleComp spec β) :
-    (liftM q >>= ob).finSupportWhen fin_poss =
-      (fin_poss q).biUnion fun x => (ob x).finSupportWhen fin_poss := by
-  simp [finSupportWhen]
+-- @[simp] lemma finSupportWhen_query_bind [DecidableEq β]
+--     (q : OracleQuery spec α) (ob : α → OracleComp spec β) :
+--     (liftM q >>= ob).finSupportWhen fin_poss =
+--       (fin_poss q).biUnion fun x => (ob x).finSupportWhen fin_poss := by
+--   simp [finSupportWhen]
 
-@[simp] lemma finSupport_query_bind [spec.FiniteRange] [Fintype α] [DecidableEq β]
-    (q : OracleQuery spec α) (ob : α → OracleComp spec β) :
-    (liftM q >>= ob).finSupport = Finset.univ.biUnion fun x => (ob x).finSupport := by
-  cases q; simp [finSupport, Finset.ext_iff]
+-- @[simp] lemma finSupport_query_bind [spec.FiniteRange] [Fintype α] [DecidableEq β]
+--     (q : OracleQuery spec α) (ob : α → OracleComp spec β) :
+--     (liftM q >>= ob).finSupport = Finset.univ.biUnion fun x => (ob x).finSupport := by
+--   cases q; simp [finSupport, Finset.ext_iff]
 
-@[simp] lemma supportWhen_bind (oa : OracleComp spec α) (ob : α → OracleComp spec β) :
-    (oa >>= ob).supportWhen poss = ⋃ x ∈ oa.supportWhen poss, (ob x).supportWhen poss := by
-  induction oa using OracleComp.inductionOn with
-  | pure _ => simp
-  | query_bind i t oa hoa => simp [hoa]
-  | failure => simp
-
-@[simp] lemma support_bind (oa : OracleComp spec α) (ob : α → OracleComp spec β) :
-    (oa >>= ob).support = ⋃ x ∈ oa.support, (ob x).support := by
-  simp [support]
-
-@[simp] lemma finSupportWhen_bind (oa : OracleComp spec α) (ob : α → OracleComp spec β)
-    [DecidableEq α] [DecidableEq β] :
-    (oa >>= ob).finSupportWhen fin_poss =
-      (oa.finSupportWhen fin_poss).biUnion fun x => (ob x).finSupportWhen fin_poss := by
-  induction oa using OracleComp.inductionOn with
-  | pure _ => simp
-  | query_bind i t oa hoa => simp [hoa, Finset.biUnion_biUnion]
-  | failure => simp
-
-@[simp] lemma finSupport_bind (oa : OracleComp spec α) (ob : α → OracleComp spec β)
-    [hα : DecidableEq α] [hβ : DecidableEq β] [spec.FiniteRange] :
-    (oa >>= ob).finSupport = oa.finSupport.biUnion (λ x ↦ (ob x).finSupport) := by
-  simp [finSupport]
-
-lemma mem_support_bind_iff (oa : OracleComp spec α) (ob : α → OracleComp spec β) (y : β) :
-    y ∈ (oa >>= ob).support ↔ ∃ x ∈ oa.support, y ∈ (ob x).support := by simp
-
-lemma mem_finSupport_bind_iff [spec.FiniteRange]
-    (oa : OracleComp spec α) (ob : α → OracleComp spec β)
-    [hoa : DecidableEq α] [hob : DecidableEq β] (y : β) : y ∈ (oa >>= ob).finSupport ↔
-      ∃ x ∈ oa.finSupport, y ∈ (ob x).finSupport := by simp
-
-/-- The support of a computation is finite if oracles have finite ranges. -/
-instance supportWhen_finite [spec.FiniteRange] (oa : OracleComp spec α) :
-    Finite ↥(oa.supportWhen poss) := by
-  induction oa using OracleComp.inductionOn with
-  | pure x => exact Set.finite_singleton x
-  | query_bind i t oa hoa =>
-      simpa using Finite.Set.finite_biUnion'' _ fun x => (oa x).supportWhen poss
-  | failure => exact Set.toFinite ∅
-
-/-- The support of a computation is finite when viewed as a type. -/
-instance support_finite [spec.FiniteRange] (oa : OracleComp spec α) :
-    Finite ↥(oa.support) := supportWhen_finite _ oa
-
-/-- With a `DecidableEq` instance we can show that the support is actually a `Fintype`,
-rather than just `Finite` as in `support_finite`. -/
-instance support_fintype [spec.FiniteRange] [DecidableEq α] (oa : OracleComp spec α) :
-    Fintype ↥oa.support := by
-  induction oa using OracleComp.construct with
-  | pure x => exact Fintype.subtypeEq x
-  | query_bind q oa hoa => have := q.rangeFintype; simpa using Set.fintypeiUnion _
-  | failure => exact Set.fintypeEmpty
-
-end basic
-
-section coe
-
-/-- `finSupport` when viewed as a `Set` gives the regular `support` of the computation.  -/
-@[simp]
-lemma coe_finSupport [spec.FiniteRange] [DecidableEq α]
-    (oa : OracleComp spec α) : ↑oa.finSupport = oa.support := by
-  induction oa using OracleComp.induction with
-  | pure x => apply Finset.coe_singleton
-  | query_bind i t oa hoa => simp [hoa]
-  | failure => apply Finset.coe_empty
-
-variable [spec.FiniteRange] [DecidableEq α] (oa : OracleComp spec α) (s : Finset α)
-
-lemma finSupport_eq_iff_support_eq_coe : oa.finSupport = s ↔ oa.support = ↑s :=
-  Finset.coe_inj.symm.trans (by rw [coe_finSupport])
-lemma eq_finSupport_iff_coe_eq_support : s = oa.finSupport ↔ ↑s = oa.support :=
-  Finset.coe_inj.symm.trans (by rw [coe_finSupport])
-
-lemma finSupport_subset_iff_support_subset_coe : oa.finSupport ⊆ s ↔ oa.support ⊆ ↑s :=
-  Finset.coe_subset.symm.trans (by rw [coe_finSupport])
-lemma subset_finSupport_iff_coe_subset_support : s ⊆ oa.finSupport ↔ ↑s ⊆ oa.support :=
-  Finset.coe_subset.symm.trans (by rw [coe_finSupport])
-
-lemma mem_finSupport_iff_mem_support (x : α) : x ∈ oa.finSupport ↔ x ∈ oa.support := by
-  rw [← Finset.mem_coe, coe_finSupport]
-
-lemma mem_finSupport_of_mem_support {x : α} (hx : x ∈ oa.support) : x ∈ oa.finSupport :=
-  (mem_finSupport_iff_mem_support oa x).2 hx
-lemma mem_support_of_mem_finSupport {x : α} (hx : x ∈ oa.finSupport) : x ∈ oa.support :=
-  (mem_finSupport_iff_mem_support oa x).1 hx
-
-end coe
-
-section decidable
-
-/-- If the output type of a computation has `DecidableEq` then membership in the `support`
-of a computation is also decidable as a predicate.
-NOTE: will need to be restricted if we allow infinite oracle codomains. -/
-instance decidablePred_mem_support [spec.FiniteRange] [hα : DecidableEq α]
-    (oa : OracleComp spec α) : DecidablePred (· ∈ oa.support) := by
-  induction oa using OracleComp.construct with
-  | pure x => exact λ y ↦ hα y x
-  | failure => exact λ _ ↦ Decidable.isFalse (not_false)
-  | query_bind q oa hoa =>
-      simp only [support_bind, support_query, Set.mem_univ, Set.iUnion_true, Set.mem_iUnion]
-      have := q.rangeFintype
-      exact λ _ ↦ Fintype.decidableExistsFintype
-
-/-- Membership in `finSupport` is a decidable predicate if it's defined. -/
-instance decidablePred_mem_finSupport [spec.DecidableEq] [spec.FiniteRange] [DecidableEq α]
-    (oa : OracleComp spec α) : DecidablePred (· ∈ oa.finSupport) := by
-  simp [mem_finSupport_iff_mem_support]
-  apply decidablePred_mem_support
-
-end decidable
-
-section nonempty
-
-variable (oa : OracleComp spec α)
-
--- lemma defaultResult_mem_support : oa.defaultResult ∈ oa.support := by
+-- @[simp] lemma supportWhen_bind (oa : OracleComp spec α) (ob : α → OracleComp spec β) :
+--     (oa >>= ob).supportWhen poss = ⋃ x ∈ oa.supportWhen poss, (ob x).supportWhen poss := by
 --   induction oa using OracleComp.inductionOn with
---   | h_pure x => simp only [defaultResult, support_pure, Set.mem_singleton_iff]
---   | h_queryBind i t oa hoa =>
---       have : ∃ u, defaultResult (oa default) ∈ (oa u).support := ⟨default, hoa default⟩
---       simpa only [defaultResult, OracleComp.bind'_eq_bind, pure_bind,support_bind,support_query,
---         Set.mem_univ, Set.iUnion_true, Set.mem_iUnion] using this
+--   | pure _ => simp
+--   | query_bind i t oa hoa => simp [hoa]
+--   | failure => simp
 
--- lemma exists_mem_support : ∃ x : α, x ∈ oa.support :=
---   ⟨defaultResult oa, defaultResult_mem_support oa⟩
+-- @[simp] lemma support_bind (oa : OracleComp spec α) (ob : α → OracleComp spec β) :
+--     (oa >>= ob).support = ⋃ x ∈ oa.support, (ob x).support := by
+--   simp [support]
 
--- lemma defaultResult_mem_finSupport [DecidableEq α] : oa.defaultResult ∈ oa.finSupport := by
---   simpa only [mem_finSupport_iff_mem_support] using defaultResult_mem_support oa
+-- @[simp] lemma finSupportWhen_bind (oa : OracleComp spec α) (ob : α → OracleComp spec β)
+--     [DecidableEq α] [DecidableEq β] :
+--     (oa >>= ob).finSupportWhen fin_poss =
+--       (oa.finSupportWhen fin_poss).biUnion fun x => (ob x).finSupportWhen fin_poss := by
+--   induction oa using OracleComp.inductionOn with
+--   | pure _ => simp
+--   | query_bind i t oa hoa => simp [hoa, Finset.biUnion_biUnion]
+--   | failure => simp
 
--- @[simp] lemma support_nonempty : oa.support.Nonempty :=
---   ⟨defaultResult oa, defaultResult_mem_support oa⟩
+-- @[simp] lemma finSupport_bind (oa : OracleComp spec α) (ob : α → OracleComp spec β)
+--     [hα : DecidableEq α] [hβ : DecidableEq β] [spec.FiniteRange] :
+--     (oa >>= ob).finSupport = oa.finSupport.biUnion (λ x ↦ (ob x).finSupport) := by
+--   simp [finSupport]
 
--- @[simp] lemma finSupport_nonempty [DecidableEq α] : oa.finSupport.Nonempty :=
---   ⟨defaultResult oa, defaultResult_mem_finSupport oa⟩
+-- lemma mem_support_bind_iff (oa : OracleComp spec α) (ob : α → OracleComp spec β) (y : β) :
+--     y ∈ (oa >>= ob).support ↔ ∃ x ∈ oa.support, y ∈ (ob x).support := by simp
 
--- @[simp] lemma support_ne_empty : oa.support ≠ ∅ := (support_nonempty oa).ne_empty
--- @[simp] lemma finSupport_ne_empty [DecidableEq α] : oa.finSupport ≠ ∅ :=
---   Finset.ne_empty_of_mem (defaultResult_mem_finSupport oa)
+-- lemma mem_finSupport_bind_iff [spec.FiniteRange]
+--     (oa : OracleComp spec α) (ob : α → OracleComp spec β)
+--     [hoa : DecidableEq α] [hob : DecidableEq β] (y : β) : y ∈ (oa >>= ob).finSupport ↔
+--       ∃ x ∈ oa.finSupport, y ∈ (ob x).finSupport := by simp
 
--- @[simp] lemma support_eq_singleton_iff (x : α) :
---     oa.support = {x} ↔ oa.support ⊆ {x} := by
---   rw [oa.support_nonempty.subset_singleton_iff]
--- @[simp] lemma finSupport_eq_singleton_iff [DecidableEq α] (x : α) :
---     oa.finSupport = {x} ↔ oa.finSupport ⊆ {x} := by
+-- /-- The support of a computation is finite if oracles have finite ranges. -/
+-- instance supportWhen_finite [spec.FiniteRange] (oa : OracleComp spec α) :
+--     Finite ↥(oa.supportWhen poss) := by
+--   induction oa using OracleComp.inductionOn with
+--   | pure x => exact Set.finite_singleton x
+--   | query_bind i t oa hoa =>
+--       simpa using Finite.Set.finite_biUnion'' _ fun x => (oa x).supportWhen poss
+--   | failure => exact Set.toFinite ∅
+
+-- /-- The support of a computation is finite when viewed as a type. -/
+-- instance support_finite [spec.FiniteRange] (oa : OracleComp spec α) :
+--     Finite ↥(oa.support) := supportWhen_finite _ oa
+
+-- /-- With a `DecidableEq` instance we can show that the support is actually a `Fintype`,
+-- rather than just `Finite` as in `support_finite`. -/
+-- instance support_fintype [spec.FiniteRange] [DecidableEq α] (oa : OracleComp spec α) :
+--     Fintype ↥oa.support := by
+--   induction oa using OracleComp.construct with
+--   | pure x => exact Fintype.subtypeEq x
+--   | query_bind q oa hoa => have := q.rangeFintype; simpa using Set.fintypeiUnion _
+--   | failure => exact Set.fintypeEmpty
+
+-- end basic
+
+-- section coe
+
+-- /-- `finSupport` when viewed as a `Set` gives the regular `support` of the computation.  -/
+-- @[simp]
+-- lemma coe_finSupport [spec.FiniteRange] [DecidableEq α]
+--     (oa : OracleComp spec α) : ↑oa.finSupport = oa.support := by
+--   induction oa using OracleComp.induction with
+--   | pure x => apply Finset.coe_singleton
+--   | query_bind i t oa hoa => simp [hoa]
+--   | failure => apply Finset.coe_empty
+
+-- variable [spec.FiniteRange] [DecidableEq α] (oa : OracleComp spec α) (s : Finset α)
+
+-- lemma finSupport_eq_iff_support_eq_coe : oa.finSupport = s ↔ oa.support = ↑s :=
+--   Finset.coe_inj.symm.trans (by rw [coe_finSupport])
+-- lemma eq_finSupport_iff_coe_eq_support : s = oa.finSupport ↔ ↑s = oa.support :=
+--   Finset.coe_inj.symm.trans (by rw [coe_finSupport])
+
+-- lemma finSupport_subset_iff_support_subset_coe : oa.finSupport ⊆ s ↔ oa.support ⊆ ↑s :=
+--   Finset.coe_subset.symm.trans (by rw [coe_finSupport])
+-- lemma subset_finSupport_iff_coe_subset_support : s ⊆ oa.finSupport ↔ ↑s ⊆ oa.support :=
+--   Finset.coe_subset.symm.trans (by rw [coe_finSupport])
+
+-- lemma mem_finSupport_iff_mem_support (x : α) : x ∈ oa.finSupport ↔ x ∈ oa.support := by
+--   rw [← Finset.mem_coe, coe_finSupport]
+
+-- lemma mem_finSupport_of_mem_support {x : α} (hx : x ∈ oa.support) : x ∈ oa.finSupport :=
+--   (mem_finSupport_iff_mem_support oa x).2 hx
+-- lemma mem_support_of_mem_finSupport {x : α} (hx : x ∈ oa.finSupport) : x ∈ oa.support :=
+--   (mem_finSupport_iff_mem_support oa x).1 hx
+
+-- end coe
+
+-- section decidable
+
+-- /-- If the output type of a computation has `DecidableEq` then membership in the `support`
+-- of a computation is also decidable as a predicate.
+-- NOTE: will need to be restricted if we allow infinite oracle codomains. -/
+-- instance decidablePred_mem_support [spec.FiniteRange] [hα : DecidableEq α]
+--     (oa : OracleComp spec α) : DecidablePred (· ∈ oa.support) := by
+--   induction oa using OracleComp.construct with
+--   | pure x => exact λ y ↦ hα y x
+--   | failure => exact λ _ ↦ Decidable.isFalse (not_false)
+--   | query_bind q oa hoa =>
+--       simp only [support_bind, support_query, Set.mem_univ, Set.iUnion_true, Set.mem_iUnion]
+--       have := q.rangeFintype
+--       exact λ _ ↦ Fintype.decidableExistsFintype
+
+-- /-- Membership in `finSupport` is a decidable predicate if it's defined. -/
+-- instance decidablePred_mem_finSupport [spec.DecidableEq] [spec.FiniteRange] [DecidableEq α]
+--     (oa : OracleComp spec α) : DecidablePred (· ∈ oa.finSupport) := by
+--   simp [mem_finSupport_iff_mem_support]
+--   apply decidablePred_mem_support
+
+-- end decidable
+
+-- section nonempty
+
+-- variable (oa : OracleComp spec α)
+
+-- -- lemma defaultResult_mem_support : oa.defaultResult ∈ oa.support := by
+-- --   induction oa using OracleComp.inductionOn with
+-- --   | h_pure x => simp only [defaultResult, support_pure, Set.mem_singleton_iff]
+-- --   | h_queryBind i t oa hoa =>
+-- --       have : ∃ u, defaultResult (oa default) ∈ (oa u).support := ⟨default, hoa default⟩
+-- --       simpa only [defaultResult, OracleComp.bind'_eq_bind, pure_bind,support_bind,support_query,
+-- --         Set.mem_univ, Set.iUnion_true, Set.mem_iUnion] using this
+
+-- -- lemma exists_mem_support : ∃ x : α, x ∈ oa.support :=
+-- --   ⟨defaultResult oa, defaultResult_mem_support oa⟩
+
+-- -- lemma defaultResult_mem_finSupport [DecidableEq α] : oa.defaultResult ∈ oa.finSupport := by
+-- --   simpa only [mem_finSupport_iff_mem_support] using defaultResult_mem_support oa
+
+-- -- @[simp] lemma support_nonempty : oa.support.Nonempty :=
+-- --   ⟨defaultResult oa, defaultResult_mem_support oa⟩
+
+-- -- @[simp] lemma finSupport_nonempty [DecidableEq α] : oa.finSupport.Nonempty :=
+-- --   ⟨defaultResult oa, defaultResult_mem_finSupport oa⟩
+
+-- -- @[simp] lemma support_ne_empty : oa.support ≠ ∅ := (support_nonempty oa).ne_empty
+-- -- @[simp] lemma finSupport_ne_empty [DecidableEq α] : oa.finSupport ≠ ∅ :=
+-- --   Finset.ne_empty_of_mem (defaultResult_mem_finSupport oa)
+
+-- -- @[simp] lemma support_eq_singleton_iff (x : α) :
+-- --     oa.support = {x} ↔ oa.support ⊆ {x} := by
+-- --   rw [oa.support_nonempty.subset_singleton_iff]
+-- -- @[simp] lemma finSupport_eq_singleton_iff [DecidableEq α] (x : α) :
+-- --     oa.finSupport = {x} ↔ oa.finSupport ⊆ {x} := by
+-- --   simp [finSupport_eq_iff_support_eq_coe]
+
+-- end nonempty
+
+-- @[simp] lemma support_eqRec (oa : OracleComp spec α) (h : α = β) :
+--     (h ▸ oa).support = h.symm ▸ oa.support := by
+--   induction h; rfl
+-- @[simp] lemma finSupport_eqRec [spec.DecidableEq] [spec.FiniteRange]
+--     [hα : DecidableEq α] [hβ : DecidableEq β] (oa : OracleComp spec α) (h : α = β) :
+--     @finSupport _ _ _ _ hβ (h ▸ oa : OracleComp spec β) =
+--       h.symm ▸ @finSupport _ _ _ _ hα oa := by
+--   refine Finset.ext (λ x ↦ ?_)
+--   simp [mem_finSupport_iff_mem_support]
+--   induction h -- We can't do this earlier without running into trouble with `DecidableEq`
+--   exact Iff.symm (mem_finSupport_iff_mem_support oa x)
+
+-- lemma mem_support_eqRec_iff (oa : OracleComp spec α) (h : α = β) (y : β) :
+--     y ∈ (h ▸ oa).support ↔ h.symm ▸ y ∈ oa.support := by
+--   induction h; rfl
+-- -- lemma mem_finSupport_eqRec_iff [spec.DecidableEq] [spec.FiniteRange]
+-- --     [hα : DecidableEq α] [hβ : DecidableEq β] (oa : OracleComp spec α) (h : α = β) (y : β) :
+-- --     y ∈ (h ▸ oa).finSupport ↔ h.symm ▸ y ∈ oa.finSupport := by
+-- --   induction h; rfl
+
+-- @[simp] lemma support_map (oa : OracleComp spec α) (f : α → β) :
+--     (f <$> oa).support = f '' oa.support := by
+--   simp only [map_eq_pure_bind, ← Set.image_eq_iUnion, support_bind, support_pure]
+-- @[simp] lemma fin_support_map [spec.DecidableEq] [spec.FiniteRange]
+--     [DecidableEq α] [DecidableEq β] (oa : OracleComp spec α) (f : α → β) :
+--     (f <$> oa).finSupport = oa.finSupport.image f := by
 --   simp [finSupport_eq_iff_support_eq_coe]
 
-end nonempty
+-- lemma mem_support_map {oa : OracleComp spec α} {x : α}
+--     (hx : x ∈ oa.support) (f : α → β) : f x ∈ (f <$> oa).support := by
+--   simp only [support_map, Set.mem_image]
+--   refine ⟨x, hx, rfl⟩
 
-@[simp] lemma support_eqRec (oa : OracleComp spec α) (h : α = β) :
-    (h ▸ oa).support = h.symm ▸ oa.support := by
-  induction h; rfl
-@[simp] lemma finSupport_eqRec [spec.DecidableEq] [spec.FiniteRange]
-    [hα : DecidableEq α] [hβ : DecidableEq β] (oa : OracleComp spec α) (h : α = β) :
-    @finSupport _ _ _ _ hβ (h ▸ oa : OracleComp spec β) =
-      h.symm ▸ @finSupport _ _ _ _ hα oa := by
-  refine Finset.ext (λ x ↦ ?_)
-  simp [mem_finSupport_iff_mem_support]
-  induction h -- We can't do this earlier without running into trouble with `DecidableEq`
-  exact Iff.symm (mem_finSupport_iff_mem_support oa x)
+-- @[simp] lemma support_ite (p : Prop) [Decidable p] (oa oa' : OracleComp spec α) :
+--     (if p then oa else oa').support = if p then oa.support else oa'.support :=
+--   apply_ite support p oa oa'
+-- @[simp] lemma finSupport_ite [spec.DecidableEq] [spec.FiniteRange] [DecidableEq α]
+--     (p : Prop) [Decidable p] (oa oa' : OracleComp spec α) :
+--     (if p then oa else oa').finSupport = if p then oa.finSupport else oa'.finSupport :=
+--   apply_ite finSupport p oa oa'
 
-lemma mem_support_eqRec_iff (oa : OracleComp spec α) (h : α = β) (y : β) :
-    y ∈ (h ▸ oa).support ↔ h.symm ▸ y ∈ oa.support := by
-  induction h; rfl
--- lemma mem_finSupport_eqRec_iff [spec.DecidableEq] [spec.FiniteRange]
---     [hα : DecidableEq α] [hβ : DecidableEq β] (oa : OracleComp spec α) (h : α = β) (y : β) :
---     y ∈ (h ▸ oa).finSupport ↔ h.symm ▸ y ∈ oa.finSupport := by
---   induction h; rfl
+-- @[simp] lemma support_coin : coin.support = {true, false} := by
+--   simpa using Set.pair_comm false true
+-- @[simp] lemma finSupport_coin : coin.finSupport = {true, false} := by
+--   simp [finSupport_eq_iff_support_eq_coe]
+--   exact Set.pair_comm false true
 
-@[simp] lemma support_map (oa : OracleComp spec α) (f : α → β) :
-    (f <$> oa).support = f '' oa.support := by
-  simp only [map_eq_pure_bind, ← Set.image_eq_iUnion, support_bind, support_pure]
-@[simp] lemma fin_support_map [spec.DecidableEq] [spec.FiniteRange]
-    [DecidableEq α] [DecidableEq β] (oa : OracleComp spec α) (f : α → β) :
-    (f <$> oa).finSupport = oa.finSupport.image f := by
-  simp [finSupport_eq_iff_support_eq_coe]
+-- @[simp] lemma support_uniformFin (n : ℕ) : ($[0..n]).support = Set.univ := support_query _
+-- @[simp] lemma finSupport_uniformFin (n : ℕ) : ($[0..n]).finSupport = Finset.univ :=
+--   finSupport_query _
 
-lemma mem_support_map {oa : OracleComp spec α} {x : α}
-    (hx : x ∈ oa.support) (f : α → β) : f x ∈ (f <$> oa).support := by
-  simp only [support_map, Set.mem_image]
-  refine ⟨x, hx, rfl⟩
+-- example : support (do
+--     let b ← coin; let b' ← coin
+--     let x ← (if b && b' then return 0 else return 1);
+--     let z ← (if b && b' then return x else return 0);
+--     return (x * z)) = {0} :=
+--   by simp [Set.eq_singleton_iff_unique_mem]
 
-@[simp] lemma support_ite (p : Prop) [Decidable p] (oa oa' : OracleComp spec α) :
-    (if p then oa else oa').support = if p then oa.support else oa'.support :=
-  apply_ite support p oa oa'
-@[simp] lemma finSupport_ite [spec.DecidableEq] [spec.FiniteRange] [DecidableEq α]
-    (p : Prop) [Decidable p] (oa oa' : OracleComp spec α) :
-    (if p then oa else oa').finSupport = if p then oa.finSupport else oa'.finSupport :=
-  apply_ite finSupport p oa oa'
-
-@[simp] lemma support_coin : coin.support = {true, false} := by
-  simpa using Set.pair_comm false true
-@[simp] lemma finSupport_coin : coin.finSupport = {true, false} := by
-  simp [finSupport_eq_iff_support_eq_coe]
-  exact Set.pair_comm false true
-
-@[simp] lemma support_uniformFin (n : ℕ) : ($[0..n]).support = Set.univ := support_query _
-@[simp] lemma finSupport_uniformFin (n : ℕ) : ($[0..n]).finSupport = Finset.univ :=
-  finSupport_query _
-
-example : support (do
-    let b ← coin; let b' ← coin
-    let x ← (if b && b' then return 0 else return 1);
-    let z ← (if b && b' then return x else return 0);
-    return (x * z)) = {0} :=
-  by simp [Set.eq_singleton_iff_unique_mem]
-
-example : finSupport (do
-    let b ← coin; let b' ← coin
-    let x ← (if b || b' then return 0 else return 1);
-    let z ← (if b || b' then return x else return 0);
-    return (x * z)) = {0} :=
-  by simp
+-- example : finSupport (do
+--     let b ← coin; let b' ← coin
+--     let x ← (if b || b' then return 0 else return 1);
+--     let z ← (if b || b' then return x else return 0);
+--     return (x * z)) = {0} :=
+--   by simp
 
 -- section simulate
 
